Add emptyable to can_finalize proof

execution/examples/BAT.v
@@ -1038,6 +1038,28 @@ Qed.
 
 (* ------------------- Constants are constant ------------------- *)
 
+Lemma receive_total_supply_increasing : forall prev_state new_state chain ctx msg new_acts,
+  ((current_slot chain) <= (fundingEnd prev_state))%nat ->
+  receive chain ctx prev_state msg = Some (new_state, new_acts) ->
+       (total_supply prev_state) <= (total_supply new_state).
+Proof.
+  intros.
+  destruct msg. destruct m. destruct m.
+  - apply try_transfer_preserves_total_supply in H0. lia.
+  - apply try_transfer_from_preserves_total_supply in H0. lia.
+  - apply try_approve_preserves_total_supply in H0. lia.
+  - apply try_create_tokens_total_supply_correct in H0.
+    rewrite <- H0. apply N.le_add_r.
+  - apply try_finalize_preserves_total_supply in H0. lia.
+  - specialize try_refund_is_some as [_ H1].
+    rewrite H0 in H1. now destruct H1; eauto.
+  - now receive_simpl.
+Qed.
+
+
+
+(* ------------------- Constants are constant ------------------- *)
+
 Lemma receive_preserves_constants : forall prev_state new_state chain ctx msg new_acts,
   receive chain ctx prev_state msg = Some (new_state, new_acts) ->
        prev_state.(fundDeposit) = new_state.(fundDeposit)
@@ -1476,22 +1498,111 @@ Proof.
     + now eapply IHaccounts.
 Qed.
 
-Lemma can_finalize_if_deployed : forall deployed_bstate (reward : Amount) (caddr creator : Address),
+Definition pending_usage bstate account : Amount :=
+  Z.min (sumZ (fun act => if address_eqb act.(act_from) account
+                         then Z.max 0 (act_amount act) 
+                         else 0%Z) bstate.(chain_state_queue))
+        (env_account_balances bstate account).
+
+Definition spendable_balance (bstate : ChainState) accounts : Amount :=
+  let account_balance := env_account_balances bstate in
+    sumZ (fun acc => account_balance acc - pending_usage bstate acc)%Z accounts.
+
+Lemma spendable_eq_total_balance : forall bstate accounts,
+  reachable bstate ->
+  chain_state_queue bstate = [] ->
+  spendable_balance bstate accounts = total_balance bstate accounts.
+Proof.
+  intros.
+  unfold spendable_balance, total_balance, pending_usage.
+  rewrite H0. cbn.
+  rewrite sumZ_map_id.
+  setoid_rewrite sumZ_map_id at 2.
+  f_equal.
+  apply map_ext_in.
+  intros.
+  rewrite Z.min_l, Z.sub_0_r; auto.
+  apply Z.ge_le.
+  now apply account_balance_nonnegative.
+Qed.
+
+Lemma spendable_consume_act : forall (bstate1 bstate2 : ChainState) accounts act acts,
+  (env_account_balances bstate1 act.(act_from) <= env_account_balances bstate2 act.(act_from) + (Z.max 0 (act_amount act)))%Z ->
+  (forall a, In a accounts -> a <> act.(act_from) -> env_account_balances bstate1 a <= env_account_balances bstate2 a)%Z ->
+  chain_state_queue bstate1 = act :: acts ->
+  chain_state_queue bstate2 = acts ->
+  (spendable_balance bstate1 accounts <= spendable_balance bstate2 accounts)%Z.
+Proof.
+  intros.
+  induction accounts.
+  - apply Z.le_refl.
+  - cbn.
+    apply Z.add_le_mono.
+    + destruct (address_eqdec a (act_from act)).
+      * rewrite e. clear e. cbn.
+        unfold pending_usage.
+        rewrite H1, H2. cbn.
+        rewrite address_eq_refl.
+        lia.
+      * apply H0 in n as h3; try apply in_eq.
+        unfold pending_usage.
+        rewrite H1, H2. cbn.
+        rewrite address_eq_ne; auto.
+        lia.
+    + apply IHaccounts.
+      intros.
+      apply H0; eauto.
+      now apply in_cons.
+Qed.
+
+Lemma spendable_balance_positive : forall bstate accounts,
+  reachable bstate ->
+  (0 <= spendable_balance bstate accounts)%Z.
+Proof.
+  intros.
+  unfold spendable_balance.
+  induction accounts.
+  - apply Z.le_refl.
+  - cbn.
+    apply Ztac.add_le.
+    + apply Zle_minus_le_0.
+      unfold pending_usage.
+      lia.
+    + apply IHaccounts.
+Qed.
+
+Lemma spendable_balance_transfer_le : forall (bstate1 bstate2 : ChainState) from to amount accounts acts,
+  (amount >= 0)%Z ->
+  EnvironmentEquiv bstate2 (transfer_balance from to amount bstate1) ->
+  chain_state_queue bstate1 = {| act_from := from; act_body := act_transfer to amount |} :: acts ->
+  chain_state_queue bstate2 = acts ->
+    (spendable_balance bstate1 accounts <= spendable_balance bstate2 accounts)%Z.
+Proof.
+  intros.
+  destruct (in_dec address_eqdec from accounts); destruct (in_dec address_eqdec to accounts);
+    try (repeat split; eauto;
+         eapply spendable_consume_act; eauto;
+           intros; rewrite_environment_equiv; cbn;
+           destruct_address_eq; try easy; lia).
+Qed.
+
+
+Lemma can_finalize_if_deployed : forall deployed_bstate (reward : Amount) (caddr creator : Address) accounts,
   address_is_contract creator = false ->
   (reward >= 0)%Z ->
-  (exists deployed_cstate accounts,
-    reachable deployed_bstate
-    /\ chain_state_queue deployed_bstate = []
-    /\ env_contracts deployed_bstate caddr = Some (BAT.contract : WeakContract)
+  reachable deployed_bstate ->
+  emptyable (chain_state_queue deployed_bstate) ->
+  NoDup accounts ->
+  Forall (fun acc => address_is_contract acc = false) accounts ->
+  (exists deployed_cstate,
+    env_contracts deployed_bstate caddr = Some (BAT.contract : WeakContract)
     /\ env_contract_states deployed_bstate caddr = Some (serializeState deployed_cstate)
     /\ (((tokenCreationMin deployed_cstate) - (total_supply deployed_cstate))) <=
-            ((Z.to_N (total_balance deployed_bstate accounts)) * (tokenExchangeRate deployed_cstate))
+            ((Z.to_N (spendable_balance deployed_bstate accounts)) * (tokenExchangeRate deployed_cstate))
     /\ deployed_cstate.(tokenExchangeRate) <= deployed_cstate.(tokenCreationCap) - deployed_cstate.(tokenCreationMin)
     /\ ((fundingStart deployed_cstate) <= (current_slot (env_chain deployed_bstate)))%nat
     /\ ((current_slot (env_chain deployed_bstate)) < (fundingEnd deployed_cstate))%nat
     /\ address_is_contract (fundDeposit deployed_cstate) = false
-    /\ NoDup accounts
-    /\ Forall (fun acc => address_is_contract acc = false) accounts
     /\ deployed_cstate.(tokenExchangeRate) <> 0)
       ->
       exists bstate, reachable_through deployed_bstate bstate
@@ -1501,127 +1612,189 @@ Lemma can_finalize_if_deployed : forall deployed_bstate (reward : Amount) (caddr
         /\ env_contract_states bstate caddr = Some (serializeState cstate)
         /\ (isFinalized cstate) = true.
 Proof.
-  intros deployed_bstate reward caddr creator Hcreator Hreward
-    [deployed_cstate [accounts [H1 [H2 [H3 [H4 [H5 [H6 [H7 [H8 [H9 [H10 [H11 H12]]]]]]]]]]]]].
-  destruct (isFinalized deployed_cstate) eqn:finalized; [eexists; split; eauto|].
+  intros deployed_bstate reward caddr creator accounts Hcreator Hreward reach empty accounts_unique accounts_not_contracts H.
+  pattern (deployed_bstate) in H.
+  eapply empty_queue in H; cycle 1; eauto.
+  - clear H Hcreator Hreward reward.
+    intros bstate bstate' act acts reach_from reach_to
+      [deployed_cstate [H1 [H2 [H3 [H4 [H5 [H6 [H7 H8]]]]]]]] queue queue' [[action_eval] | env_eq]; only 1: destruct_action_eval.
+    + exists deployed_cstate.
+      repeat split; eauto;
+        try (rewrite_environment_equiv; cbn; (easy || now destruct_address_eq)).
+      eapply N.le_trans.
+      apply H3.
+      apply N.mul_le_mono_r, Z2N.inj_le; try now apply spendable_balance_positive.
+      eapply spendable_consume_act; eauto;
+        intros; rewrite_environment_equiv; subst;
+        cbn; destruct_address_eq; try easy; lia.
+    + exists deployed_cstate.
+      repeat split; eauto;
+        try (rewrite_environment_equiv; cbn; (easy || now destruct_address_eq)).
+      eapply N.le_trans.
+      apply H3.
+      apply N.mul_le_mono_r, Z2N.inj_le; try now apply spendable_balance_positive.
+      eapply spendable_consume_act; eauto;
+        intros; rewrite_environment_equiv; subst;
+        cbn; destruct_address_eq; try easy; lia.
+    + destruct (address_eqdec caddr to_addr).
+      * rewrite e5 in *.
+        rewrite H1 in e. inversion e. rewrite <- H0 in *.
+        rewrite H2 in e0. inversion e0. rewrite <- H9 in *.
+        apply wc_receive_strong in e2 as [prev_state' [msg' [new_state' [H16 [H17 [H18 H19]]]]]].
+        rewrite deserialize_serialize in H16. inversion H16. rewrite H10 in *.
+        apply receive_total_supply_increasing in H19 as total_supply_increasing; try (cbn; lia).
+        apply receive_preserves_constants in H19 as (H20 & H21 & H22 & H23 & H24 & H45 & H26).
+        repeat match goal with
+        | H : _ prev_state' =  _ new_state' |- _=> rewrite H in *; clear H
+        end.
+        eexists new_state'.
+        repeat split; eauto;
+          try (rewrite_environment_equiv; cbn; (easy || now destruct_address_eq)).
+        eapply N.le_trans in H3; [| apply N.sub_le_mono_l, total_supply_increasing].
+        eapply N.le_trans.
+        apply H3.
+        apply N.mul_le_mono_r, Z2N.inj_le; try now apply spendable_balance_positive.
+        eapply spendable_consume_act; eauto;
+          intros; rewrite_environment_equiv; subst; destruct msg;
+          cbn; destruct_address_eq; try easy; lia.
+      * exists deployed_cstate.
+        repeat split; eauto;
+          try (rewrite_environment_equiv; cbn; (easy || now destruct_address_eq)).
+        eapply N.le_trans.
+        apply H3.
+        apply N.mul_le_mono_r, Z2N.inj_le; try now apply spendable_balance_positive.
+        eapply spendable_consume_act; eauto;
+          intros; rewrite_environment_equiv; subst; destruct msg;
+          cbn; destruct_address_eq; try easy; lia.
+    + exists deployed_cstate.
+      repeat split; eauto; try (rewrite_environment_equiv; cbn; easy).
+      eapply N.le_trans.
+      apply H3.
+      apply N.mul_le_mono_r, Z2N.inj_le; try now apply spendable_balance_positive.
+      eapply spendable_consume_act; eauto; intros; rewrite_environment_equiv; lia.
+  - destruct H as (bstate & (reach' & (cstate & H1 & H2 & H3 & H4 & H5 & H6 & H7 & H8) & queue)).
+    update_all.
+    rewrite spendable_eq_total_balance in H3; eauto.
 
-  add_block (create_token_acts (deployed_bstate<|env_account_balances := add_balance creator reward deployed_bstate.(env_account_balances)|>) caddr accounts
-          ((tokenCreationMin deployed_cstate) - (total_supply deployed_cstate)) deployed_cstate.(tokenExchangeRate)) 1%nat;
-    only 1: apply Hcreator; eauto; [now apply All_Forall.In_Forall, create_token_acts_is_account | ].
-  update ((current_slot bstate) <= (fundingEnd deployed_cstate))%nat in H8 by
-    (rewrite_environment_equiv; cbn; lia).
-  update (setter_from_getter_Environment_env_account_balances
-             (fun _ : Address -> Amount => add_balance creator reward (env_account_balances deployed_bstate)) deployed_bstate)
-    with bstate.(chain_state_env) in queue by
-    (rewrite queue; apply create_token_acts_eq; intros; now rewrite_environment_equiv).
-  update deployed_bstate with bstate in H5.
-  { eapply N.le_trans; eauto.
-    apply N.mul_le_mono_r, Z2N.inj_le;
-      try now apply total_balance_positive.
-    apply (total_balance_le deployed_bstate).
-    intros. rewrite_environment_equiv. cbn.
-    destruct_address_eq; lia.
-  }
-  update_all.
-  generalize dependent bstate.
-  generalize dependent deployed_cstate.
+    destruct (isFinalized cstate) eqn:finalized; [eexists; split; eauto|].
 
-  induction accounts; intros.
-  - apply N.le_0_r, N.sub_0_le in H5.
-    specialize (can_finalize_if_creation_min bstate reward caddr creator).
-    intros []; eauto.
-  - apply NoDup_cons_iff in H10 as [H10 H10'].
-    apply list.Forall_cons in H11 as [H11 H11'].
-    destruct (tokenCreationMin deployed_cstate - total_supply deployed_cstate) eqn:tokens_left_to_fund.
-    + eapply IHaccounts; eauto.
-      * now rewrite tokens_left_to_fund.
-      * rewrite tokens_left_to_fund.
-        apply N.le_0_l.
-    + rewrite <- tokens_left_to_fund in *.
-      clear Hreward.
-      destruct (0 <? env_account_balances bstate a)%Z eqn:balance_positive; cycle 1;
-        [apply Z.ltb_ge in balance_positive | apply Z.ltb_lt in balance_positive].
-      { assert (amount_zero : (forall x, x <= 0 -> Z.to_N x = 0%N)%Z) by lia.
-        rewrite create_token_acts_cons, amount_zero, N.min_0_r, N.mul_0_l, N.sub_0_r in queue by lia.
-        discard_invalid_action; eauto.
-        - intros.
-          destruct_action_eval;
-          [inversion e0 | inversion e1 | destruct msg; inversion e1; subst].
-          rewrite H3 in e. inversion e. subst.
-          apply wc_receive_strong in e2 as [prev_state' [msg' [new_state' [H16 [H17 [H18 H19]]]]]].
-          destruct_match in H17; try congruence.
-          cbn in H17.
-          rewrite deserialize_serialize in H17.
-          inversion H17. subst.
-          now apply try_create_tokens_amount_correct in H19.
-        - edestruct IHaccounts with (bstate := bstate0) (deployed_cstate := deployed_cstate); eauto; try (rewrite_environment_equiv; eauto).
-          + rewrite queue0.
-            apply create_token_acts_eq.
-            intros. now rewrite_environment_equiv.
-          + rewrite total_balance_distr, N.add_comm in H5; eauto.
-            erewrite (total_balance_eq _ bstate) by (intros; now rewrite_environment_equiv).
-            lia.
-          + destruct H as [H H'].
-            now exists x.
-      }
+    add_block (create_token_acts (bstate<|env_account_balances := add_balance creator reward bstate.(env_account_balances)|>) caddr accounts
+            ((tokenCreationMin cstate) - (total_supply cstate)) cstate.(tokenExchangeRate)) 1%nat;
+      only 1: apply Hcreator; eauto; [now apply All_Forall.In_Forall, create_token_acts_is_account | ].
+    update ((current_slot bstate0) <= (fundingEnd cstate))%nat in H6 by
+      (rewrite_environment_equiv; cbn; lia).
+    update (setter_from_getter_Environment_env_account_balances
+               (fun _ : Address -> Amount => add_balance creator reward (env_account_balances bstate)) bstate)
+      with bstate0.(chain_state_env) in queue0 by
+      (rewrite queue0; apply create_token_acts_eq; intros; now rewrite_environment_equiv).
+    update bstate with bstate0 in H3.
+    { eapply N.le_trans; eauto.
+      apply N.mul_le_mono_r, Z2N.inj_le;
+        try now apply total_balance_positive.
+      apply (total_balance_le bstate).
+      intros. rewrite_environment_equiv. cbn.
+      destruct_address_eq; lia.
+    }
+    update_all.
+    generalize dependent bstate0.
+    generalize dependent cstate.
 
-      evaluate_action BAT.contract; try easy.
-      * now rewrite create_token_acts_cons by lia.
-      * apply Z.le_ge, N2Z.is_nonneg.
-      * nia.
-      * apply Nat.ltb_ge in H7.
-        apply Nat.ltb_ge in H8.
-        cbn.
-        rewrite finalized, H7, H8, N2Z.inj_min, Z2N.id;
-        try (apply Z.ge_le, account_balance_nonnegative; eauto).
-        cbn.
-        destruct_match eqn:match_amount; returnIf match_amount.
-        destruct_match eqn:match_cap; returnIf match_cap.
-        -- eauto.
-        -- apply N.ltb_lt in match_cap.
-           apply Z.leb_gt, Z.min_glb_lt_iff in match_amount as [].
-           rewrite Z2N.inj_min, N2Z.id, <- N.mul_min_distr_r, <- N.add_min_distr_l, N.min_glb_lt_iff in match_cap.
-           destruct match_cap.
-           apply N.lt_le_trans with (p := (tokenCreationMin deployed_cstate) + tokenExchangeRate deployed_cstate) in H1.
-           nia.
-           rewrite N.mul_add_distr_r, N.mul_1_l.
-           rewrite N.add_assoc, N.add_comm, N.add_assoc.
-           rewrite <- N.add_le_mono_r.
-           apply N_le_sub. lia.
-           now apply N_div_mul_le.
-        -- apply Zle_bool_imp_le, Z.min_le in match_amount as [].
-         --- rewrite <- N2Z.inj_0 in H.
-             now apply N2Z.inj_le, N_le_add_distr in H.
-         --- lia.
-      * assert (caddr_not_in_accounts : ~ In caddr accounts) by
-          (intro; rewrite Forall_forall in H11'; apply H11' in H; now apply contract_addr_format in H3).
-        assert (env_balances_eq : forall a, In a accounts -> env_account_balances bstate0 a = env_account_balances bstate a)
-          by (intros; rewrite_environment_equiv; cbn; now destruct_address_eq).
-        edestruct IHaccounts;
-          only 12: (rewrite deployed_state; eauto);
-          try (rewrite_environment_equiv; eauto);
-          cbn; try rewrite Z2N.inj_min, N2Z.id.
-        -- rewrite queue0, N.sub_add_distr.
-           apply create_token_acts_eq.
-           intros. rewrite_environment_equiv. cbn. now destruct_address_eq.
-        -- edestruct N.min_dec.
-          --- cbn. rewrite e.
-             eapply N.le_trans; [| apply N.le_0_l].
+    induction accounts; intros.
+    + apply N.le_0_r, N.sub_0_le in H3.
+      specialize (can_finalize_if_creation_min bstate0 reward caddr creator).
+      intros []; eauto.
+    + apply NoDup_cons_iff in accounts_unique as [accounts_unique accounts_unique'].
+      apply list.Forall_cons in accounts_not_contracts as [accounts_not_contracts accounts_not_contracts'].
+      destruct (tokenCreationMin cstate - total_supply cstate) eqn:tokens_left_to_fund.
+      * eapply IHaccounts; eauto.
+       -- now rewrite tokens_left_to_fund.
+       -- rewrite tokens_left_to_fund.
+          apply N.le_0_l.
+      * rewrite <- tokens_left_to_fund in *.
+        clear Hreward.
+        destruct (0 <? env_account_balances bstate0 a)%Z eqn:balance_positive; cycle 1;
+          [apply Z.ltb_ge in balance_positive | apply Z.ltb_lt in balance_positive].
+        { assert (amount_zero : (forall x, x <= 0 -> Z.to_N x = 0%N)%Z) by lia.
+          rewrite create_token_acts_cons, amount_zero, N.min_0_r, N.mul_0_l, N.sub_0_r in queue0 by lia.
+          discard_invalid_action; eauto.
+          - intros.
+            destruct_action_eval;
+            [inversion e0 | inversion e1 | destruct msg; inversion e1; subst].
+            rewrite H1 in e. inversion e. subst.
+            apply wc_receive_strong in e2 as [prev_state' [msg' [new_state' [H16 [H17 [H18 H19]]]]]].
+            destruct_match in H17; try congruence.
+            cbn in H17.
+            rewrite deserialize_serialize in H17.
+            inversion H17. subst.
+            now apply try_create_tokens_amount_correct in H19.
+          - edestruct IHaccounts with (bstate0 := bstate) (cstate := cstate); eauto; try (rewrite_environment_equiv; eauto).
+            + rewrite queue.
+              apply create_token_acts_eq.
+              intros. now rewrite_environment_equiv.
+            + rewrite total_balance_distr, N.add_comm in H3; eauto.
+              erewrite (total_balance_eq _ bstate0) by (intros; now rewrite_environment_equiv).
+              lia.
+            + destruct H as [H H'].
+              now exists x.
+        }
+
+        evaluate_action BAT.contract; try easy.
+        -- now rewrite create_token_acts_cons by lia.
+        -- apply Z.le_ge, N2Z.is_nonneg.
+        -- nia.
+        -- apply Nat.ltb_ge in H5.
+           apply Nat.ltb_ge in H6.
+           cbn.
+           rewrite finalized, H5, H6, N2Z.inj_min, Z2N.id;
+             try (apply Z.ge_le, account_balance_nonnegative; eauto).
+           cbn.
+           destruct_match eqn:match_amount; returnIf match_amount.
+           destruct_match eqn:match_cap; returnIf match_cap; eauto.
+         --- apply N.ltb_lt in match_cap.
+             apply Z.leb_gt, Z.min_glb_lt_iff in match_amount as [].
+             rewrite Z2N.inj_min, N2Z.id, <- N.mul_min_distr_r, <- N.add_min_distr_l, N.min_glb_lt_iff in match_cap.
+             destruct match_cap.
+             apply N.lt_le_trans with (p := (tokenCreationMin cstate) + tokenExchangeRate cstate) in H9.
+             nia.
              rewrite N.mul_add_distr_r, N.mul_1_l.
-             apply N.le_0_r.
-             rewrite N.sub_add_distr.
-             rewrite N.sub_add_distr.
-             apply N.sub_0_le.
-             now apply N_le_div_mul.
-          --- rewrite total_balance_distr, N.add_comm in H5; eauto.
-             erewrite total_balance_eq by auto.
-             apply N.le_sub_le_add_r in H5.
-             rewrite <- N.sub_add_distr in H5.
-             eapply N.le_trans; [| apply H5].
-             apply N.sub_le_mono_l, N.add_le_mono_l, N.mul_le_mono_r.
-             lia.
-        -- destruct H as [H H'].
-           now exists x.
+             rewrite N.add_assoc, N.add_comm, N.add_assoc.
+             rewrite <- N.add_le_mono_r.
+             apply N_le_sub. lia.
+             now apply N_div_mul_le.
+         --- apply Zle_bool_imp_le, Z.min_le in match_amount as [].
+          ---- rewrite <- N2Z.inj_0 in H.
+               now apply N2Z.inj_le, N_le_add_distr in H.
+          ---- lia.
+        -- assert (caddr_not_in_accounts : ~ In caddr accounts) by
+             (intro; rewrite Forall_forall in accounts_not_contracts'; apply accounts_not_contracts' in H; now apply contract_addr_format in H1).
+           assert (env_balances_eq : forall a, In a accounts -> env_account_balances bstate0 a = env_account_balances bstate a)
+             by (intros; rewrite_environment_equiv; cbn; now destruct_address_eq).
+           edestruct IHaccounts;
+             only 12: (rewrite deployed_state; eauto);
+             try (rewrite_environment_equiv; eauto);
+             cbn; try rewrite Z2N.inj_min, N2Z.id.
+         --- rewrite queue, N.sub_add_distr.
+             apply create_token_acts_eq.
+             intros. rewrite_environment_equiv. cbn. now destruct_address_eq.
+         --- edestruct N.min_dec.
+          ---- cbn. rewrite e.
+               eapply N.le_trans; [| apply N.le_0_l].
+               rewrite N.mul_add_distr_r, N.mul_1_l.
+               apply N.le_0_r.
+               rewrite N.sub_add_distr.
+               rewrite N.sub_add_distr.
+               apply N.sub_0_le.
+               now apply N_le_div_mul.
+          ---- rewrite total_balance_distr, N.add_comm in H3; eauto.
+               erewrite (total_balance_eq _ bstate0) by
+                (intros; rewrite_environment_equiv; cbn; now destruct_address_eq).
+               apply N.le_sub_le_add_r in H3.
+               rewrite <- N.sub_add_distr in H3.
+               eapply N.le_trans; [| apply H3].
+               apply N.sub_le_mono_l, N.add_le_mono_l, N.mul_le_mono_r.
+               lia.
+         --- destruct H as [H H'].
+             now exists x.
 Qed.
 
 End Theories.
